progress backedge elimination

BoogieLang/BackedgeElim.thy
@@ -1,13 +1,6 @@
 theory BackedgeElim
-imports Semantics Util
+imports Semantics Util "HOL-Eisbach.Eisbach" "HOL-Eisbach.Eisbach_Tools"
 begin
-
-fun mods_contained_in :: "vname set \<Rightarrow> cmd list \<Rightarrow> bool"
-  where
-    "mods_contained_in H [] = True"
-  | "mods_contained_in H ((Havoc h)#cs) = ((h \<notin> H) \<and> mods_contained_in H cs)"
-  | "mods_contained_in H ((Assign x e)#cs) = ((x \<notin> H) \<and> mods_contained_in H cs)"
-  | "mods_contained_in H (c#cs) = mods_contained_in H cs"
 
 definition nstate_same_on :: "var_context \<Rightarrow> 'a nstate \<Rightarrow> 'a nstate \<Rightarrow> vname set \<Rightarrow> bool"
   where "nstate_same_on \<Lambda> ns1 ns2 D = ((\<forall>d. d \<notin> D \<longrightarrow> lookup_var \<Lambda> ns1 d = lookup_var \<Lambda> ns2 d) \<and> 
@@ -15,6 +8,10 @@ definition nstate_same_on :: "var_context \<Rightarrow> 'a nstate \<Rightarrow> 
                                             old_global_state ns1 = old_global_state ns2)"
 
 lemma nstate_same_on_empty: "nstate_same_on \<Lambda> ns1 ns1 {}"
+  unfolding nstate_same_on_def
+  by simp
+
+lemma nstate_same_on_sym: "nstate_same_on \<Lambda> ns1 ns2 D \<Longrightarrow> nstate_same_on \<Lambda> ns2 ns1 D"
   unfolding nstate_same_on_def
   by simp
 
@@ -105,12 +102,48 @@ definition state_well_typed :: "'a absval_ty_fun \<Rightarrow> var_context \<Rig
          (\<forall>x \<tau>. lookup_var_ty \<Lambda> x = Some \<tau> \<longrightarrow>
              (\<exists>v. lookup_var \<Lambda> ns x = Some v \<and> type_of_val A v = instantiate \<Omega> \<tau>))"
 
+lemma state_wt_nstate_same_on:
+  assumes "state_well_typed A \<Lambda> \<Omega> ns1" and "nstate_same_on \<Lambda> ns1 ns2 {}"
+  shows "state_well_typed A \<Lambda> \<Omega> ns2"
+  using assms 
+  unfolding state_well_typed_def nstate_same_on_def
+  by simp
+
+
 fun is_method_call :: "cmd \<Rightarrow> bool"
   where
     "is_method_call (MethodCall m args rets) = True"
   | "is_method_call _ = False"
 
-(* TODO: nat argument may be redundant *)
+lemma red_cmd_state_wt_preserve:
+  assumes "A,M,\<Lambda>,\<Gamma>,\<Omega> \<turnstile> \<langle>c, Normal ns\<rangle> \<rightarrow> Normal ns'" and "state_well_typed A \<Lambda> \<Omega> ns" and "\<not> (is_method_call c)"
+  shows "state_well_typed A \<Lambda> \<Omega> ns'"
+  using assms
+  by (cases) (auto simp: state_well_typed_def)
+
+lemma normal_reduce_aux:
+  assumes "A,M,\<Lambda>,\<Gamma>,\<Omega> \<turnstile> \<langle>c, Normal ns\<rangle> \<rightarrow> s''" and "A,M,\<Lambda>,\<Gamma>,\<Omega> \<turnstile> \<langle>cs, s''\<rangle> [\<rightarrow>] Normal ns'"
+  shows "\<exists>ns''. s'' = Normal ns''"
+  using assms
+  using failure_stays_cmd_list magic_stays_cmd_list state.exhaust by blast
+
+lemma red_cmds_state_wt_preserve_aux:
+  assumes "A,M,\<Lambda>,\<Gamma>,\<Omega> \<turnstile> \<langle>cs, s\<rangle> [\<rightarrow>] s'" and "s = Normal ns" and "s' = Normal ns'" and
+          "state_well_typed A \<Lambda> \<Omega> ns" and "list_all (\<lambda>c. \<not> (is_method_call c)) cs"
+  shows "state_well_typed A \<Lambda> \<Omega> ns'"
+  using assms
+  apply (induction arbitrary: ns ns')
+   apply simp
+  using red_cmd_state_wt_preserve normal_reduce_aux
+  by (metis list_all_simps(1))
+
+lemma red_cmds_state_wt_preserve:
+  assumes "A,M,\<Lambda>,\<Gamma>,\<Omega> \<turnstile> \<langle>cs, Normal ns\<rangle> [\<rightarrow>] Normal ns'"
+          "state_well_typed A \<Lambda> \<Omega> ns" and "list_all (\<lambda>c. \<not> (is_method_call c)) cs"
+  shows "state_well_typed A \<Lambda> \<Omega> ns'"
+  using assms red_cmds_state_wt_preserve_aux
+  by blast
+
 inductive cfg_dag_rel :: "bool \<Rightarrow> vname list \<Rightarrow> expr list \<Rightarrow> expr list \<Rightarrow> cmd list \<Rightarrow> cmd list \<Rightarrow> bool"
   for "cut_edge" :: bool
   where      
@@ -135,7 +168,13 @@ inductive cfg_dag_rel :: "bool \<Rightarrow> vname list \<Rightarrow> expr list 
    | DagRel_CutEdge:
      "cut_edge \<Longrightarrow> cfg_dag_rel cut_edge [] [] [] [] [Assume (Lit (LBool False))]"
 
-(* TODO: also need that ns1 is well-typed *)
+method cfg_dag_rel_tac_single uses R_def R_old_def LocVar_assms = 
+  (match conclusion in                       
+                       "cfg_dag_rel ?cut_edge [] [] ?post_invs (?c#?cs1) (?c#?cs2)" \<Rightarrow> \<open>rule DagRel_Main, simp\<close> \<bar>
+                       "cfg_dag_rel ?cut_edge [] [] [] [] [Assume (Lit (LBool False))]" \<Rightarrow> \<open>rule DagRel_CutEdge, simp\<close> \<bar>
+                       "cfg_dag_rel ?cut_edge ?H ?pre_invs ?post_invs ?cs1 ?cs2" \<Rightarrow> \<open>rule\<close> \<bar>
+                       "_" \<Rightarrow> fail)
+
 lemma cfg_dag_rel_havoc:
   assumes "cfg_dag_rel c H pre_invs post_invs cs1 cs2" and
           "nstate_same_on \<Lambda> ns1 ns2 (set H)" and
@@ -170,39 +209,6 @@ proof (induction arbitrary: ns2)
     using RedCmdListCons apply fastforce
     using RelRest by simp
 qed (auto intro: RedCmdListNil cfg_dag_rel.intros)
-
-lemma assume_red_true:
-  assumes "A,M,\<Lambda>,\<Gamma>,\<Omega> \<turnstile> \<langle>Assume e, Normal ns\<rangle> \<rightarrow> s2" and "A,\<Lambda>,\<Gamma>,\<Omega> \<turnstile> \<langle>e, ns\<rangle> \<Down> BoolV True"
-  shows "s2 = Normal ns"
-  using assms
-  apply cases
-  by (auto dest: expr_eval_determ(1))
-
-lemma assume_red_false:
-  assumes "A,M,\<Lambda>,\<Gamma>,\<Omega> \<turnstile> \<langle>Assume e, Normal ns\<rangle> \<rightarrow> s2" and "A,\<Lambda>,\<Gamma>,\<Omega> \<turnstile> \<langle>e, ns\<rangle> \<Down> BoolV False"
-  shows "s2 = Magic"
-  using assms
-  apply cases
-  by (auto dest: expr_eval_determ(1))
-
-lemma assume_determ:
-  assumes "A,M,\<Lambda>,\<Gamma>,\<Omega> \<turnstile> \<langle>Assume e, s1\<rangle> \<rightarrow> s2" and "A,M,\<Lambda>,\<Gamma>,\<Omega> \<turnstile> \<langle>Assume e, s1\<rangle> \<rightarrow> s3"
-  shows "s2 = s3"
-  using assms
-proof (cases s1)
-  case (Normal ns)
-  then show ?thesis 
-  proof (cases "A,\<Lambda>,\<Gamma>,\<Omega> \<turnstile> \<langle>e, ns\<rangle> \<Down> BoolV True")
-    case True
-    then show ?thesis using assms Normal 
-      using assume_red_true by blast
-  next
-    case False
-    then show ?thesis using assms Normal 
-      by (metis assume_cases_ext)
-  qed
-qed (auto dest: failure_stays_cmd magic_stays_cmd)
-
 
 lemma cfg_dag_rel_pre_invs:
   assumes "cfg_dag_rel c H pre_invs post_invs cs1 cs2" and
@@ -316,8 +322,8 @@ next
   show ?case
     apply (rule exI[where ?x="[]"])
     using DagRel_Main
-         by (auto intro: RedCmdListNil cfg_dag_rel.DagRel_Main)
-     qed (auto intro: RedCmdListNil cfg_dag_rel.intros simp: nstate_same_on_def)
+      by (auto intro: RedCmdListNil cfg_dag_rel.DagRel_Main)
+qed (auto intro: RedCmdListNil cfg_dag_rel.intros simp: nstate_same_on_def)
 
 lemma red_cmd_nstate_same_on:
   assumes "A,M,\<Lambda>,\<Gamma>,\<Omega> \<turnstile> \<langle>c, Normal ns1\<rangle> \<rightarrow> s'" and
@@ -352,17 +358,16 @@ next
     using red_cmd.RedHavoc by blast
 qed (simp)
 
-
 lemma cfg_dag_rel_same:
   assumes "cfg_dag_rel c H pre_invs post_invs cs1 cs2" and
           "H = []" and
           "pre_invs = []" and
-          "A,M,\<Lambda>,\<Gamma>,\<Omega> \<turnstile> \<langle>cs1, Normal ns1\<rangle> [\<rightarrow>] s'" and
+          "A,M,\<Lambda>,\<Gamma>,\<Omega> \<turnstile> \<langle>cs1, Normal ns1\<rangle> [\<rightarrow>] s'" and         
           "nstate_same_on \<Lambda> ns1 ns2 {}" and
           "\<And> s2'. A,M,\<Lambda>,\<Gamma>,\<Omega> \<turnstile> \<langle>cs2, Normal ns2\<rangle> [\<rightarrow>] s2' \<Longrightarrow> s2' \<noteq> Failure"
   shows "\<exists>cs2A cs2B. cs2 = cs2A@cs2B \<and>   
     s' \<noteq> Failure \<and> 
-    (\<forall>ns'. s' = Normal ns1' \<longrightarrow> (\<exists>ns2'. nstate_same_on \<Lambda> ns1' ns2' {} \<and> cfg_dag_rel c [] [] post_invs [] cs2B \<and> (A,M,\<Lambda>,\<Gamma>,\<Omega> \<turnstile> \<langle>cs2A, Normal ns2\<rangle> [\<rightarrow>] Normal ns2')))"
+    (\<forall>ns1'. s' = Normal ns1' \<longrightarrow> (\<exists>ns2'. nstate_same_on \<Lambda> ns1' ns2' {} \<and> cfg_dag_rel c [] [] post_invs [] cs2B \<and> (A,M,\<Lambda>,\<Gamma>,\<Omega> \<turnstile> \<langle>cs2A, Normal ns2\<rangle> [\<rightarrow>] Normal ns2')))"
   using assms
 proof (induction arbitrary: ns1 ns2)
   case (DagRel_Main cmd post_invs cs1 cs2)
@@ -378,13 +383,13 @@ proof (induction arbitrary: ns1 ns2)
       using DagRel_Main.prems(5) RedCmdListCons by blast
     with DagRel_Main.IH RedCs1 Normal \<open>nstate_same_on \<Lambda> ns1'' ns2'' {}\<close> obtain cs2A cs2B where 
      Rec:"cs2 = cs2A @ cs2B" "s' \<noteq> Failure" 
-         "\<forall>ns'. s' = Normal ns1' \<longrightarrow> (\<exists>ns2'. nstate_same_on \<Lambda> ns1' ns2' {} \<and> cfg_dag_rel c [] [] post_invs [] cs2B \<and> A,M,\<Lambda>,\<Gamma>,\<Omega> \<turnstile> \<langle>cs2A,Normal ns2''\<rangle> [\<rightarrow>] Normal ns2')"
+         "\<forall>ns1'. s' = Normal ns1' \<longrightarrow> (\<exists>ns2'. nstate_same_on \<Lambda> ns1' ns2' {} \<and> cfg_dag_rel c [] [] post_invs [] cs2B \<and> A,M,\<Lambda>,\<Gamma>,\<Omega> \<turnstile> \<langle>cs2A,Normal ns2''\<rangle> [\<rightarrow>] Normal ns2')"
       by metis    
     show ?thesis 
       apply (rule exI[where ?x = "(cmd)#cs2A"])
       apply (rule exI[where ?x = "cs2B"])
       using Rec RedCmd2 
-      by (auto intro: RedCmdListCons)      
+      by (metis RedCmdListCons append_Cons)      
   next
     case Failure
     then show ?thesis 
@@ -406,121 +411,300 @@ next
     by (metis RedCmdListNil append.left_neutral cfg_dag_rel.DagRel_CutEdge nil_cmd_elim state.distinct(1) state.inject)
 qed (auto intro: RedCmdListNil cfg_dag_rel.intros)
 
-
 lemma cfg_dag_rel_post_invs:
-  assumes "cfg_dag_rel c [] [] post_invs [] cs2" and
-          "\<And> s2'. A,M,\<Lambda>,\<Gamma>,\<Omega> \<turnstile> \<langle>cs2, Normal ns\<rangle> [\<rightarrow>] s2' \<Longrightarrow> s2' \<noteq> Failure"
+  assumes "cfg_dag_rel c H pre_invs post_invs cs1 cs2" and
+          "H = []" and "pre_invs = []" and "cs1 = []"
+          "\<And> s2'. A,M,\<Lambda>,\<Gamma>,\<Omega> \<turnstile> \<langle>cs2, Normal ns\<rangle> [\<rightarrow>] s2' \<Longrightarrow> s2' \<noteq> Failure" and
+          "list_all (\<lambda>inv. \<exists>b. A,\<Lambda>,\<Gamma>,\<Omega> \<turnstile> \<langle>inv, ns\<rangle> \<Down> BoolV b) post_invs"
   shows "\<exists> cs2A cs2B.  cs2 = cs2A@cs2B \<and> 
     cfg_dag_rel c [] [] [] [] cs2B \<and> 
     (A,M,\<Lambda>,\<Gamma>,\<Omega> \<turnstile> \<langle>cs2A, Normal ns\<rangle> [\<rightarrow>] Normal ns) \<and>
     list_all (expr_sat A \<Lambda> \<Gamma> \<Omega> ns) post_invs"
   using assms
 proof induction
+  case (DagRel_PostInv post_invs cs2 e_inv)
+  from this obtain b where "A,\<Lambda>,\<Gamma>,\<Omega> \<turnstile> \<langle>e_inv,ns\<rangle> \<Down> (BoolV b)" by auto
+  with DagRel_PostInv obtain s'' where Red1:"A,M,\<Lambda>,\<Gamma>,\<Omega> \<turnstile> \<langle>Assert e_inv, Normal ns\<rangle> \<rightarrow> s''"
+    by (metis (full_types) RedAssertFail RedAssertOk)
+  hence Normal:"s'' = Normal ns" using \<open>\<And>s2'. A,M,\<Lambda>,\<Gamma>,\<Omega> \<turnstile> \<langle>Assert e_inv # cs2,Normal ns\<rangle> [\<rightarrow>] s2' \<Longrightarrow> s2' \<noteq> Failure\<close>
+    by (metis (full_types) RedAssertFail RedCmdListCons \<open>A,\<Lambda>,\<Gamma>,\<Omega> \<turnstile> \<langle>e_inv,ns\<rangle> \<Down> BoolV b\<close> assert_correct failure_red_cmd_list)
+  with Red1 DagRel_PostInv obtain cs2A cs2B where
+    Rec:"cs2 = cs2A @ cs2B \<and> cfg_dag_rel c [] [] [] [] cs2B \<and> (A,M,\<Lambda>,\<Gamma>,\<Omega> \<turnstile> \<langle>cs2A,Normal ns\<rangle> [\<rightarrow>] Normal ns) \<and> list_all (expr_sat A \<Lambda> \<Gamma> \<Omega> ns) post_invs"
+    by (metis RedCmdListCons list.pred_inject(2))
+  show ?case
+    apply (rule exI[where ?x="Assert e_inv # cs2A"])
+    apply (rule exI[where ?x=cs2B])
+    using Red1 Normal Rec 
+    unfolding expr_sat_def 
+    by (auto intro: RedCmdListCons)
+qed (auto intro: RedCmdListNil cfg_dag_rel.intros)
 
-
+lemma cfg_dag_rel_no_method_calls:
+  assumes "cfg_dag_rel c H pre_invs post_invs cs1 cs2"
+  shows "list_all (\<lambda>c. \<not> is_method_call c) cs2"
+  using assms
+  by (induction) auto
+ 
 lemma dag_rel_block_lemma:
   assumes Red:"A,M,\<Lambda>,\<Gamma>,\<Omega> \<turnstile> \<langle>cs1, Normal ns1\<rangle> [\<rightarrow>] s'" and
           InvsHold:"list_all (expr_sat A \<Lambda> \<Gamma> \<Omega> ns1) pre_invs" and
           DagVerifies:"\<And>s2'. A,M,\<Lambda>,\<Gamma>,\<Omega> \<turnstile> \<langle>cs2, Normal ns2\<rangle> [\<rightarrow>] s2' \<Longrightarrow> s2' \<noteq> Failure" and
           SameModH:"nstate_same_on \<Lambda> ns1 ns2 (set H)" and
-          Rel:"cfg_dag_rel c H pre_invs post_invs cs1 cs2"
-  shows "s' \<noteq> Failure \<and> (\<forall>ns'. s' = Normal ns' \<longrightarrow> list_all (expr_sat A \<Lambda> \<Gamma> \<Omega> ns') post_invs \<and> (\<not>c \<longrightarrow> (A,M,\<Lambda>,\<Gamma>,\<Omega> \<turnstile> \<langle>cs2, Normal ns2\<rangle> [\<rightarrow>] Normal ns')))"
+          Rel:"cfg_dag_rel c H pre_invs post_invs cs1 cs2" and
+          StateWt:"state_well_typed A \<Lambda> \<Omega> ns1" and
+          TyExists:"list_all (\<lambda>x. lookup_var_ty \<Lambda> x \<noteq> None) H" and
+          PostInvsReduce: "\<And>ns. state_well_typed A \<Lambda> \<Omega> ns \<Longrightarrow> list_all (\<lambda>inv. \<exists>b. A,\<Lambda>,\<Gamma>,\<Omega> \<turnstile> \<langle>inv, ns\<rangle> \<Down> BoolV b) post_invs"
+        shows "s' \<noteq> Failure \<and> 
+              (\<forall>ns1'. s' = Normal ns1' \<longrightarrow> list_all (expr_sat A \<Lambda> \<Gamma> \<Omega> ns1') post_invs \<and> 
+                 (\<exists>ns2'. nstate_same_on \<Lambda> ns1' ns2' {} \<and> (\<not>c \<longrightarrow> (A,M,\<Lambda>,\<Gamma>,\<Omega> \<turnstile> \<langle>cs2, Normal ns2\<rangle> [\<rightarrow>] Normal ns2'))))"
 proof -
-  from cfg_dag_rel_havoc[OF Rel SameModH] obtain cs2A cs2B where
-    "cs2 = cs2A@cs2B" and A2Red1:"A,M,\<Lambda>,\<Gamma>,\<Omega> \<turnstile> \<langle>cs2A, Normal ns2\<rangle> [\<rightarrow>] Normal ns1" and RelHavoc:"cfg_dag_rel c [] pre_invs post_invs cs1 cs2B"
+  from cfg_dag_rel_havoc[OF Rel SameModH StateWt TyExists] obtain cs2A cs2B ns2' where
+    "cs2 = cs2A@cs2B" and StateRel1:"nstate_same_on \<Lambda> ns1 ns2' {}" and A2Red1:"A,M,\<Lambda>,\<Gamma>,\<Omega> \<turnstile> \<langle>cs2A, Normal ns2\<rangle> [\<rightarrow>] Normal ns2'"
+    and RelHavoc:"cfg_dag_rel c [] pre_invs post_invs cs1 cs2B"
     by meson
 
-  from cfg_dag_rel_pre_invs[OF RelHavoc Red InvsHold] obtain cs1A cs1B cs2A' cs2B' where
-    "cs1 = cs1A@cs1B" and "cs2B = cs2A'@cs2B'" and RelPreInvs:"cfg_dag_rel c [] [] post_invs cs1B cs2B'" and
-    A1Red1:"(A,M,\<Lambda>,\<Gamma>,\<Omega> \<turnstile> \<langle>cs1A, Normal ns1\<rangle> [\<rightarrow>] Normal ns1)" and A1Red2:"(A,M,\<Lambda>,\<Gamma>,\<Omega> \<turnstile> \<langle>cs1B, Normal ns1\<rangle> [\<rightarrow>] s')" and 
-    A2Red2:"(A,M,\<Lambda>,\<Gamma>,\<Omega> \<turnstile> \<langle>cs2A', Normal ns1\<rangle> [\<rightarrow>] Normal ns1)" 
+  from cfg_dag_rel_pre_invs[OF RelHavoc _ Red StateRel1 InvsHold] obtain cs1A cs1B cs2A' cs2B' s'' where
+    "cs1 = cs1A@cs1B" and "cs2B = cs2A'@cs2B'" and 
+    A1Red1:"(A,M,\<Lambda>,\<Gamma>,\<Omega> \<turnstile> \<langle>cs1A, Normal ns1\<rangle> [\<rightarrow>] s'')" and A1Red2:"(A,M,\<Lambda>,\<Gamma>,\<Omega> \<turnstile> \<langle>cs1B, s''\<rangle> [\<rightarrow>] s')" and
+    "s'' \<noteq> Failure" and
+    NotMagic1:"(s'' \<noteq> Magic \<longrightarrow> s'' = Normal ns1 \<and> cfg_dag_rel c [] [] post_invs cs1B cs2B' \<and> A,M,\<Lambda>,\<Gamma>,\<Omega> \<turnstile> \<langle>cs2A',Normal ns2'\<rangle> [\<rightarrow>] Normal ns2')"
     by metis
 
-  from A2Red1 A2Red2 have A2Red3:"A,M,\<Lambda>,\<Gamma>,\<Omega> \<turnstile> \<langle>cs2A@cs2A',Normal ns2\<rangle> [\<rightarrow>] Normal ns1"
-    using red_cmd_list_append by blast
-
-  have "cs2 = (cs2A@cs2A')@cs2B'" using \<open>cs2 = cs2A@cs2B\<close> and \<open>cs2B = cs2A'@cs2B'\<close> by simp
-  with A2Red3 have DagVerifies2:"\<And>s2'. A,M,\<Lambda>,\<Gamma>,\<Omega> \<turnstile> \<langle>cs2B', Normal ns1\<rangle> [\<rightarrow>] s2' \<Longrightarrow> s2' \<noteq> Failure"
-    using DagVerifies red_cmd_list_append
-    by blast
-
-  from cfg_dag_rel_same[OF RelPreInvs A1Red2 DagVerifies2] obtain cs2A'' cs2B''
-    where "cs2B' = cs2A'' @ cs2B''" and RelSame:"cfg_dag_rel c [] [] post_invs [] cs2B''" and
-     "s' \<noteq> Failure" and  NormalSame:"(A,M,\<Lambda>,\<Gamma>,\<Omega> \<turnstile> \<langle>cs2A'',Normal ns1\<rangle> [\<rightarrow>] s')"
-    by blast
-
   show ?thesis
-  proof (rule conjI[OF \<open>s' \<noteq> Failure\<close>], rule allI, rule impI)
-    fix ns'
-    assume "s' = Normal ns'"
-    hence A2Red4:"A,M,\<Lambda>,\<Gamma>,\<Omega> \<turnstile> \<langle>cs2A'',Normal ns1\<rangle> [\<rightarrow>] Normal ns'" using NormalSame
+  proof (cases "s'' = Magic")
+    case True
+    then show ?thesis using A1Red2
+      using magic_stays_cmd_list by blast
+  next
+    case False
+    hence "s'' = Normal ns1" and RelPreInvs:"cfg_dag_rel c [] [] post_invs cs1B cs2B'" and 
+          A2Red2:"A,M,\<Lambda>,\<Gamma>,\<Omega> \<turnstile> \<langle>cs2A',Normal ns2'\<rangle> [\<rightarrow>] Normal ns2'"
+      using NotMagic1
+      by auto
+    hence A1Red2Normal:"(A,M,\<Lambda>,\<Gamma>,\<Omega> \<turnstile> \<langle>cs1B, Normal ns1\<rangle> [\<rightarrow>] s')" using A1Red2 by simp
+   
+    from A2Red1 A2Red2 have A2Red3:"A,M,\<Lambda>,\<Gamma>,\<Omega> \<turnstile> \<langle>cs2A@cs2A',Normal ns2\<rangle> [\<rightarrow>] Normal ns2'"
+      using red_cmd_list_append by blast
+    have "cs2 = (cs2A@cs2A')@cs2B'" using \<open>cs2 = cs2A@cs2B\<close> and \<open>cs2B = cs2A'@cs2B'\<close> by simp
+    with A2Red3 have DagVerifies2:"\<And>s2'. A,M,\<Lambda>,\<Gamma>,\<Omega> \<turnstile> \<langle>cs2B', Normal ns2'\<rangle> [\<rightarrow>] s2' \<Longrightarrow> s2' \<noteq> Failure"
+      using DagVerifies red_cmd_list_append
       by blast
-    with \<open>cs2B' = cs2A'' @ cs2B''\<close>
-    have DagVerifies3: "\<And>s2'. A,M,\<Lambda>,\<Gamma>,\<Omega> \<turnstile> \<langle>cs2B'', Normal ns'\<rangle> [\<rightarrow>] s2' \<Longrightarrow> s2' \<noteq> Failure"
-    using DagVerifies2  red_cmd_list_append
-    by blast
-      
-    from cfg_dag_rel_post_invs[OF RelSame DagVerifies3] obtain cs2A''' cs2B'''
-      where "cs2B'' = cs2A''' @ cs2B'''" and
-      RelPostInv:"cfg_dag_rel c [] [] [] [] cs2B'''" and
-      A2Red5:"(A,M,\<Lambda>,\<Gamma>,\<Omega> \<turnstile> \<langle>cs2A''', Normal ns'\<rangle> [\<rightarrow>] Normal ns')" and
-      PostInvsHold:"list_all (expr_sat A \<Lambda> \<Gamma> \<Omega> ns') post_invs"
-      by metis
+    
+    from cfg_dag_rel_same[OF RelPreInvs _ _ A1Red2Normal StateRel1 DagVerifies2]  obtain cs2A'' cs2B''
+      where "cs2B' = cs2A'' @ cs2B''" 
+       "s' \<noteq> Failure" and
+       Normal1:"(\<forall>ns1'. s' = Normal ns1' \<longrightarrow> (\<exists>ns2'a. nstate_same_on \<Lambda> ns1' ns2'a {} \<and> cfg_dag_rel c [] [] post_invs [] cs2B'' \<and> A,M,\<Lambda>,\<Gamma>,\<Omega> \<turnstile> \<langle>cs2A'',Normal ns2'\<rangle> [\<rightarrow>] Normal ns2'a))"
+      by blast
   
-    show "list_all (expr_sat A \<Lambda> \<Gamma> \<Omega> ns') post_invs \<and> (\<not> c \<longrightarrow> A,M,\<Lambda>,\<Gamma>,\<Omega> \<turnstile> \<langle>cs2,Normal ns2\<rangle> [\<rightarrow>] Normal ns')"
-    proof (rule conjI[OF PostInvsHold], rule impI)
-      assume "\<not>c"
-      with RelPostInv have "cs2B''' = []"
-        by (cases) auto
-      with \<open>cs2 = (cs2A@cs2A')@cs2B'\<close> \<open>cs2B' = cs2A'' @ cs2B''\<close> \<open>cs2B'' = cs2A''' @ cs2B'''\<close>  A2Red3 A2Red4 A2Red5
-      show "A,M,\<Lambda>,\<Gamma>,\<Omega> \<turnstile> \<langle>cs2,Normal ns2\<rangle> [\<rightarrow>] Normal ns'"  
-        using red_cmd_list_append
-        by (metis append_Nil2)
+    show ?thesis
+    proof (rule conjI[OF \<open>s' \<noteq> Failure\<close>], rule allI, rule impI)
+      fix ns'
+      assume "s' = Normal ns'"
+        
+      from this obtain ns2'' where 
+        StateRel2:"nstate_same_on \<Lambda> ns' ns2'' {}" and RelSame:"cfg_dag_rel c [] [] post_invs [] cs2B''" and 
+        A2Red4:"A,M,\<Lambda>,\<Gamma>,\<Omega> \<turnstile> \<langle>cs2A'',Normal ns2'\<rangle> [\<rightarrow>] Normal ns2''"
+        using Normal1 by auto
+  
+      with \<open>cs2B' = cs2A'' @ cs2B''\<close>
+      have DagVerifies3: "\<And>s2'. A,M,\<Lambda>,\<Gamma>,\<Omega> \<turnstile> \<langle>cs2B'', Normal ns2''\<rangle> [\<rightarrow>] s2' \<Longrightarrow> s2' \<noteq> Failure"
+      using DagVerifies2 red_cmd_list_append
+      by blast
+  
+      have "list_all (\<lambda>c. \<not> is_method_call c) cs2" using cfg_dag_rel_no_method_calls[OF Rel] by simp
+      hence NoMethodCallPrefix:"list_all (\<lambda>c. \<not> is_method_call c) ((cs2A @ cs2A')@cs2A'')"
+        using \<open>cs2 = (cs2A@cs2A')@cs2B'\<close> \<open>cs2B' = cs2A'' @ cs2B''\<close>
+        by simp
+      from A2Red3 A2Red4 have "A,M,\<Lambda>,\<Gamma>,\<Omega> \<turnstile> \<langle>(cs2A @ cs2A')@cs2A'',Normal ns2\<rangle> [\<rightarrow>] Normal ns2''"
+        using red_cmd_list_append by blast
+      from StateWt and StateRel1 have "state_well_typed A \<Lambda> \<Omega> ns2'" 
+        using state_wt_nstate_same_on by blast
+      with A2Red4 NoMethodCallPrefix have StateWt2:"state_well_typed A \<Lambda> \<Omega> ns2''"
+        using list_all_append red_cmds_state_wt_preserve_aux by blast
+        
+      from cfg_dag_rel_post_invs[OF RelSame _ _ _ DagVerifies3 PostInvsReduce[OF StateWt2]] obtain cs2A''' cs2B'''
+        where "cs2B'' = cs2A''' @ cs2B'''" and
+        RelPostInv:"cfg_dag_rel c [] [] [] [] cs2B'''" and
+        A2Red5:"(A,M,\<Lambda>,\<Gamma>,\<Omega> \<turnstile> \<langle>cs2A''', Normal ns2''\<rangle> [\<rightarrow>] Normal ns2'')" and
+        PostInvsHold:"list_all (expr_sat A \<Lambda> \<Gamma> \<Omega> ns2'') post_invs"
+        by blast
+      have "list_all (expr_sat A \<Lambda> \<Gamma> \<Omega> ns') post_invs" 
+        apply (rule List.List.list.pred_mono_strong)
+        apply (rule PostInvsHold)
+        unfolding expr_sat_def
+        using StateRel2 eval_nstate_same_on(1) nstate_same_on_sym by blast
+     
+      show "list_all (expr_sat A \<Lambda> \<Gamma> \<Omega> ns') post_invs \<and> ((\<exists>ns2'. nstate_same_on \<Lambda> ns' ns2' {} \<and> (\<not> c \<longrightarrow> A,M,\<Lambda>,\<Gamma>,\<Omega> \<turnstile> \<langle>cs2,Normal ns2\<rangle> [\<rightarrow>] Normal ns2')))"
+      proof (rule conjI[OF _ exI])
+        show "list_all (expr_sat A \<Lambda> \<Gamma> \<Omega> ns') post_invs" 
+          apply (rule List.List.list.pred_mono_strong)
+          apply (rule PostInvsHold)
+          unfolding expr_sat_def
+          using StateRel2 eval_nstate_same_on(1) nstate_same_on_sym by blast
+      next
+        from RelPostInv have "\<not>c \<Longrightarrow> cs2B''' = []"
+          by (cases) auto
+        show "nstate_same_on \<Lambda> ns' ns2'' {} \<and> (\<not> c \<longrightarrow> A,M,\<Lambda>,\<Gamma>,\<Omega> \<turnstile> \<langle>cs2,Normal ns2\<rangle> [\<rightarrow>] Normal ns2'')"
+          apply (rule conjI[OF StateRel2])
+          apply (rule impI)
+          using  \<open>cs2 = (cs2A@cs2A')@cs2B'\<close> \<open>cs2B' = cs2A'' @ cs2B''\<close> \<open>cs2B'' = cs2A''' @ cs2B'''\<close>  A2Red3 A2Red4 A2Red5
+          by (metis \<open>\<not> c \<Longrightarrow> cs2B''' = []\<close> append.right_neutral red_cmd_list_append)
+        qed
+      qed
     qed
   qed
-qed
 
 definition dag_lemma_assms :: "'a absval_ty_fun \<Rightarrow> method_context \<Rightarrow> var_context \<Rightarrow> 
                    'a fun_interp \<Rightarrow> rtype_env \<Rightarrow> vname list \<Rightarrow> expr list \<Rightarrow> expr list \<Rightarrow>
-                   cmd list \<Rightarrow> cmd list \<Rightarrow> 'a nstate \<Rightarrow> 'a nstate \<Rightarrow> bool \<Rightarrow> bool"
-  where "dag_lemma_assms A M \<Lambda> \<Gamma> \<Omega> H pre_invs post_invs cs1 cs2 ns1 ns2 c \<equiv> 
+                    cmd list \<Rightarrow> 'a nstate \<Rightarrow> 'a nstate \<Rightarrow> bool"
+  where "dag_lemma_assms A M \<Lambda> \<Gamma> \<Omega> H pre_invs post_invs cs2 ns1 ns2 \<equiv> 
          (list_all (expr_sat A \<Lambda> \<Gamma> \<Omega> ns1) pre_invs) \<and>
          (\<forall>s2'. (A,M,\<Lambda>,\<Gamma>,\<Omega> \<turnstile> \<langle>cs2, Normal ns2\<rangle> [\<rightarrow>] s2') \<longrightarrow> s2' \<noteq> Failure) \<and>
-          (nstate_same_on \<Lambda> ns1 ns2 (set H))"
+          (nstate_same_on \<Lambda> ns1 ns2 (set H)) \<and>
+          state_well_typed A \<Lambda> \<Omega> ns1"
+
+definition dag_lemma_cfg_assms :: "'a absval_ty_fun \<Rightarrow> method_context \<Rightarrow> var_context \<Rightarrow> 
+                   'a fun_interp \<Rightarrow> rtype_env \<Rightarrow> mbodyCFG \<Rightarrow> vname list \<Rightarrow> expr list \<Rightarrow> expr list \<Rightarrow>
+                    node \<Rightarrow> 'a nstate \<Rightarrow> 'a nstate \<Rightarrow> bool"
+  where "dag_lemma_cfg_assms A M \<Lambda> \<Gamma> \<Omega> G H pre_invs post_invs m ns1 ns2 \<equiv> 
+         (list_all (expr_sat A \<Lambda> \<Gamma> \<Omega> ns1) pre_invs) \<and>
+         (\<forall>m2' s2'. (A,M,\<Lambda>,\<Gamma>,\<Omega>,G \<turnstile> (Inl m, Normal ns2) -n\<rightarrow>* (m2', s2')) \<longrightarrow> s2' \<noteq> Failure) \<and>
+          (nstate_same_on \<Lambda> ns1 ns2 (set H)) \<and>
+          state_well_typed A \<Lambda> \<Omega> ns1"
+
+lemma dag_verifies_propagate:
+  assumes "(\<And>m2' s2'. (A,M,\<Lambda>,\<Gamma>,\<Omega>,G \<turnstile> (Inl m, Normal ns) -n\<rightarrow>* (m2', s2')) \<Longrightarrow> s2' \<noteq> Failure)" and
+          "node_to_block G ! m = cs" and
+          "A,M,\<Lambda>,\<Gamma>,\<Omega> \<turnstile> \<langle>cs, Normal ns\<rangle> [\<rightarrow>] Normal ns'"
+  shows "(\<And>msuc.  List.member (out_edges(G) ! m) msuc \<Longrightarrow>
+                (\<And> m3 s3. ((A,M,\<Lambda>,\<Gamma>,\<Omega>,G \<turnstile> (Inl(msuc), Normal ns') -n\<rightarrow>* (m3, s3)) \<longrightarrow> s3 \<noteq> Failure)))"
+  sorry
+
+lemma dag_verifies_propgate_2:
+  assumes CfgVerifies:"(\<And>m2' s2'. A,M,\<Lambda>,\<Gamma>,\<Omega>,G \<turnstile> (Inl m, Normal ns) -n\<rightarrow>* (m2', s2') \<Longrightarrow> s2' \<noteq> Failure)" and
+          Block:"node_to_block G ! m = cs" and
+          BlockNormal:"A,M,\<Lambda>,\<Gamma>,\<Omega> \<turnstile> \<langle>cs,Normal ns\<rangle> [\<rightarrow>] s'"
+        shows "s' \<noteq> Failure"
+  using assms
+proof (cases "(out_edges G) ! m = []")
+  case True
+  hence "A,M,\<Lambda>,\<Gamma>,\<Omega>,G \<turnstile> (Inl m, Normal ns) -n\<rightarrow> (Inr (), s')"
+    apply (cases s')
+    using Block BlockNormal
+    by (auto intro: red_cfg.intros)
+  then show ?thesis using CfgVerifies by blast
+next
+  case False
+  from this obtain msuc where "List.member (out_edges G ! m) msuc"
+    by (metis list.exhaust member_rec(1))
+  hence "\<exists>m'. A,M,\<Lambda>,\<Gamma>,\<Omega>,G \<turnstile> (Inl m, Normal ns) -n\<rightarrow> (m', s')"
+    apply (cases s')
+    using Block BlockNormal
+    by (auto intro: red_cfg.intros)
+  thus ?thesis using CfgVerifies by blast
+qed
+
+lemma dag_lemma_assms_convert:
+  assumes "dag_lemma_cfg_assms A M \<Lambda> \<Gamma> \<Omega> G2 H pre_invs post_invs m2 ns1 ns2" and
+          "node_to_block G2 ! m2 = cs2"
+  shows "dag_lemma_assms A M \<Lambda> \<Gamma> \<Omega> H pre_invs post_invs cs2 ns1 ns2"
+  using assms
+  unfolding dag_lemma_assms_def dag_lemma_cfg_assms_def 
+  using dag_verifies_propgate_2
+  by blast
 
 definition dag_lemma_conclusion :: "'a absval_ty_fun \<Rightarrow> method_context \<Rightarrow> var_context \<Rightarrow> 
                    'a fun_interp \<Rightarrow> rtype_env \<Rightarrow> expr list \<Rightarrow>
-                   cmd list \<Rightarrow> cmd list \<Rightarrow> 'a nstate \<Rightarrow> 'a nstate \<Rightarrow> 'a state \<Rightarrow> bool \<Rightarrow> bool"
-  where "dag_lemma_conclusion A M \<Lambda> \<Gamma> \<Omega> post_invs cs1 cs2 ns1 ns2 s' c \<equiv>
-          s' \<noteq> Failure \<and> 
-         (\<forall>ns'. s' = Normal ns' \<longrightarrow> list_all (expr_sat A \<Lambda> \<Gamma> \<Omega> ns') post_invs \<and> 
-               (\<not>c \<longrightarrow> (A,M,\<Lambda>,\<Gamma>,\<Omega> \<turnstile> \<langle>cs2, Normal ns2\<rangle> [\<rightarrow>] Normal ns'))
-         )"
+                    cmd list \<Rightarrow> 'a nstate \<Rightarrow> 'a state \<Rightarrow> bool \<Rightarrow> bool"
+  where "dag_lemma_conclusion A M \<Lambda> \<Gamma> \<Omega> post_invs cs2 ns2 s' c \<equiv>
+               s' \<noteq> Failure \<and> 
+              (\<forall>ns1'. s' = Normal ns1' \<longrightarrow> list_all (expr_sat A \<Lambda> \<Gamma> \<Omega> ns1') post_invs \<and> 
+                 (\<exists>ns2'. nstate_same_on \<Lambda> ns1' ns2' {} \<and> (\<not>c \<longrightarrow> (A,M,\<Lambda>,\<Gamma>,\<Omega> \<turnstile> \<langle>cs2, Normal ns2\<rangle> [\<rightarrow>] Normal ns2'))))"
 
 lemma dag_rel_block_lemma_compact:
   assumes "A,M,\<Lambda>,\<Gamma>,\<Omega> \<turnstile> \<langle>cs1, Normal ns1\<rangle> [\<rightarrow>] s'" and
-          "dag_lemma_assms A M \<Lambda> \<Gamma> \<Omega> H pre_invs post_invs cs1 cs2 ns1 ns2 c" and
-          "cfg_dag_rel c H pre_invs post_invs cs1 cs2"
-  shows "dag_lemma_conclusion A M \<Lambda> \<Gamma> \<Omega> post_invs cs1 cs2 ns1 ns2 s' c"
+          "dag_lemma_assms A M \<Lambda> \<Gamma> \<Omega> H pre_invs post_invs cs2 ns1 ns2" and
+          "cfg_dag_rel c H pre_invs post_invs cs1 cs2" and
+          "list_all (\<lambda>x. lookup_var_ty \<Lambda> x \<noteq> None) H" and
+          "\<And>ns. state_well_typed A \<Lambda> \<Omega> ns \<Longrightarrow> list_all (\<lambda>inv. \<exists>b. A,\<Lambda>,\<Gamma>,\<Omega> \<turnstile> \<langle>inv, ns\<rangle> \<Down> BoolV b) post_invs"
+  shows "dag_lemma_conclusion A M \<Lambda> \<Gamma> \<Omega> post_invs cs2 ns2 s' c"
   using assms
   unfolding dag_lemma_assms_def dag_lemma_conclusion_def
   using dag_rel_block_lemma
   by blast
 
-lemma cfg_dag_rel_lemma_no_havoc_no_cut:
-  assumes Red:"A,M,\<Lambda>,\<Gamma>,\<Omega> \<turnstile> \<langle>cs1, Normal ns1\<rangle> [\<rightarrow>] s'" and
-          InvsHold:"list_all (expr_sat A \<Lambda> \<Gamma> \<Omega> ns1) pre_invs" and
-          DagVerifies:"\<And>s2'. A,M,\<Lambda>,\<Gamma>,\<Omega> \<turnstile> \<langle>cs2, Normal ns1\<rangle> [\<rightarrow>] s2' \<Longrightarrow> s2' \<noteq> Failure" and
-          Rel:"cfg_dag_rel False [] pre_invs post_invs cs1 cs2"
-        shows "s' \<noteq> Failure \<and> 
-              (\<forall>ns'. s' = Normal ns' \<longrightarrow> list_all (expr_sat A \<Lambda> \<Gamma> \<Omega> ns') post_invs \<and> 
-                 (A,M,\<Lambda>,\<Gamma>,\<Omega> \<turnstile> \<langle>cs2, Normal ns1\<rangle> [\<rightarrow>] Normal ns'))"
+fun mods_contained_in :: "vname set \<Rightarrow> cmd list \<Rightarrow> bool"
+  where
+    "mods_contained_in H [] = True"
+  | "mods_contained_in H ((Havoc h)#cs) = ((h \<notin> H) \<and> mods_contained_in H cs)"
+  | "mods_contained_in H ((Assign x e)#cs) = ((x \<notin> H) \<and> mods_contained_in H cs)"
+(* method calls are already desugared in this phase *)
+  | "mods_contained_in H ((MethodCall _ _ _)#cs) = False"
+  | "mods_contained_in H (c#cs) = mods_contained_in H cs"
+
+lemma mods_contained_in:
+  assumes "mods_contained_in D cs" and
+          "A,M,\<Lambda>,\<Gamma>,\<Omega> \<turnstile> \<langle>cs, s\<rangle> [\<rightarrow>] s'" and
+          "s = Normal ns" and "s' = Normal ns'"
+  shows "nstate_same_on \<Lambda> ns ns' D"
   oops
 
-lemma cfg_dag_rel_lemma_basic:
-  assumes Red:"A,M,\<Lambda>,\<Gamma>,\<Omega> \<turnstile> \<langle>cs1, Normal ns1\<rangle> [\<rightarrow>] s'" and
-          DagVerifies:"\<And>s2'. A,M,\<Lambda>,\<Gamma>,\<Omega> \<turnstile> \<langle>cs1, Normal ns1\<rangle> [\<rightarrow>] s2' \<Longrightarrow> s2' \<noteq> Failure" 
-  shows "s' \<noteq> Failure \<and> (\<forall>ns'. s' = Normal ns' \<longrightarrow> (A,M,\<Lambda>,\<Gamma>,\<Omega> \<turnstile> \<langle>cs2, Normal ns1\<rangle> [\<rightarrow>] Normal ns'))"
-  oops
+
+lemma cfg_dag_helper:
+  assumes
+   Red: "A,M,\<Lambda>,\<Gamma>,\<Omega>,G1 \<turnstile> (Inl m1, (Normal  ns1)) -n\<rightarrow>^j (m', s')" and
+   Block: "node_to_block G1 ! m1 = cs1" and
+   Block2: "node_to_block G2 ! m2 = cs2" and 
+   DagCfgAssm: "dag_lemma_cfg_assms A M \<Lambda> \<Gamma> \<Omega> G2 H pre_invs post_invs m2 ns1 ns2" and
+   BlockCorrect: "\<And> s1''. A,M,\<Lambda>,\<Gamma>,\<Omega> \<turnstile> \<langle>cs1, Normal ns1\<rangle> [\<rightarrow>] s1'' \<Longrightarrow> 
+               dag_lemma_assms A M \<Lambda> \<Gamma> \<Omega> H pre_invs post_invs cs2 ns1 ns2  \<Longrightarrow>      
+              dag_lemma_conclusion A M \<Lambda> \<Gamma> \<Omega> post_invs cs2 ns2 s1'' c" and
+(* TODO: maybe two lemmas, one where c is false and one where c is true *)
+   SuccCorrect:"\<And> msuc s4 m4 ns1'' ns2'' j'.
+            j = Suc j' \<Longrightarrow>
+            List.member (out_edges(G1) ! m1) msuc \<Longrightarrow>
+            list_all (expr_sat A \<Lambda> \<Gamma> \<Omega> ns1'') post_invs \<Longrightarrow>
+            nstate_same_on \<Lambda> ns1'' ns2'' {} \<Longrightarrow>
+            (\<not>c \<longrightarrow> (\<forall>msuc2.  List.member (out_edges(G2) ! m2) msuc2 \<longrightarrow>
+                (\<forall>m3 s3. ((A,M,\<Lambda>,\<Gamma>,\<Omega>,G2 \<turnstile> (Inl(msuc2), Normal ns2'') -n\<rightarrow>* (m3, s3)) \<longrightarrow> s3 \<noteq> Failure)))) \<Longrightarrow>
+            A,M,\<Lambda>,\<Gamma>,\<Omega>,G1 \<turnstile> (Inl(msuc), Normal ns1'') -n\<rightarrow>^j (m4, s4) \<Longrightarrow> s4 \<noteq> Failure"
+shows "s' \<noteq> Failure"
+  using assms
+proof (cases rule: relpowp_E2_2[OF assms(1)])
+  case 1
+  then show ?thesis by auto
+next
+  case (2 a b j')
+  from DagCfgAssm have DagBlockAssm:"dag_lemma_assms A M \<Lambda> \<Gamma> \<Omega> H pre_invs post_invs cs2 ns1 ns2"
+    using Block2 dag_lemma_assms_convert by blast
+  from \<open>A,M,\<Lambda>,\<Gamma>,\<Omega>,G1 \<turnstile> (Inl m1, Normal ns1) -n\<rightarrow> (a, b)\<close> show ?thesis
+  proof (cases rule: red_cfg.cases)
+    case (RedNormalSucc cs ns1'' msuc)
+    hence "dag_lemma_conclusion A M \<Lambda> \<Gamma> \<Omega> post_invs cs2 ns2 (Normal ns1'') c"
+      by (simp add: Block BlockCorrect DagBlockAssm)
+    thm dag_lemma_conclusion_def
+    from this obtain ns2'' where
+      PostHolds:"list_all (expr_sat A \<Lambda> \<Gamma> \<Omega> ns1'') post_invs" and 
+      StateRel:"nstate_same_on \<Lambda> ns1'' ns2'' {}" and
+      NormalDag:"\<not>c \<longrightarrow> A,M,\<Lambda>,\<Gamma>,\<Omega> \<turnstile> \<langle>cs2, Normal ns2\<rangle> [\<rightarrow>] Normal ns2''"
+      unfolding dag_lemma_conclusion_def
+      by blast
+    show ?thesis
+      apply (rule SuccCorrect[OF \<open>j = Suc j'\<close> \<open>List.member (out_edges G1 ! m1) msuc\<close> PostHolds StateRel])
+      apply (rule impI, rule allI, rule impI, rule allI, rule allI, rule impI)
+
+    then show ?thesis sorry
+  next
+  case (RedNormalReturn cs ns')
+    then show ?thesis using 2 finished_remains 
+  next
+    case (RedFailure cs)
+    then show ?thesis using 2 BlockCorrect Block 
+  next
+    case (RedMagic cs)
+    then show ?thesis using 2 finished_remains 
+  qed
+qed
+
 
 end
